Util/Nat/NatUtil.v
@@ -12,7 +12,7 @@ useful definitions and lemmas on natural numbers
 Set Implicit Arguments.
 
 Require Import LogicUtil Min Max Morphisms Psatz.
-Require Export Arith.
+Require Export Arith Omega.
 
 (***********************************************************************)
 (** Declare implicit arguments. *)
