Makefile
@@ -22,7 +22,7 @@ config Makefile.coq:
 
 clean:
 	rm -f `find . -name \*~`
-	$(MAKECOQ) clean
+	-$(MAKECOQ) clean
 	rm -rf `find . -name .coq-native -o -name .\*.aux -o -name \*.time -o -name \*.cache`
 
 clean-dep:
